src/tls/Test.HSL.Transcript.fst
@@ -1,0 +1,455 @@
+module Test.HSL.Transcript
+module HT = HSL.Transcript
+module Receive = HSL.Receive
+module LP = LowParse.Low.Base
+module B = LowStar.Monotonic.Buffer
+
+let preorder : LP.srel LP.byte = Ghost.hide (LowStar.Buffer.trivial_preorder LP.byte)
+
+assume
+val input: LP.slice preorder preorder
+
+open FStar.Integers
+noeq
+type flight_ch = {
+  begin_ch: uint_32;
+  ch_msg: Ghost.erased Parsers.ClientHello.clientHello
+}
+
+module HS = FStar.HyperStack
+module HSM = Parsers.Handshake
+
+let valid_flight_ch
+  = fun (flt:flight_ch) (flight_begin flight_end:uint_32) (input: LP.slice preorder preorder) (h:HS.mem) ->
+      flight_begin < flt.begin_ch /\ flt.begin_ch < flight_end /\
+      LP.valid_pos HSM.handshake_parser h input flight_begin flight_end /\
+      LP.valid_pos Parsers.ClientHello.clientHello_parser h input flt.begin_ch flight_end /\
+      (let msg = LP.contents HSM.handshake_parser h input flight_begin in
+       HSM.M_client_hello? msg /\
+       Ghost.reveal flt.ch_msg == (HSM.M_client_hello?._0 msg))
+
+open FStar.HyperStack.ST
+assume
+val receive_client_hello
+   (from to : uint_32)
+ : Stack flight_ch
+    (requires fun h -> True)
+    (ensures fun h0 fch h1 ->
+      B.modifies B.loc_none h0 h1 /\
+      valid_flight_ch fch from to input h1
+    )
+
+assume
+val output: o:LP.slice preorder preorder{
+  B.loc_disjoint (LP.loc_slice_from o 0ul)
+                 (LP.loc_slice_from input 0ul)
+  }
+
+noeq
+type flight_sh = {
+  begin_hsm:uint_32;
+  begin_sh: uint_32;
+  end_sh: uint_32;
+  sh_msg: Ghost.erased Parsers.ServerHello.serverHello
+}
+
+unfold
+let valid_flight_sh
+  = fun (flt:flight_sh) (output: LP.slice preorder preorder) (h:HS.mem) ->
+      flt.begin_hsm <= flt.begin_sh /\
+      flt.begin_sh < flt.end_sh /\
+      LP.valid_pos HSM.handshake_parser h output flt.begin_hsm flt.end_sh /\
+      LP.valid_pos Parsers.ServerHello.serverHello_parser h output flt.begin_sh flt.end_sh /\
+      (let msg = LP.contents HSM.handshake_parser h output flt.begin_hsm in
+       HSM.M_server_hello? msg /\
+       Ghost.reveal flt.sh_msg == HSM.M_server_hello?._0 msg)
+
+assume
+val nego (ch: flight_ch)
+  : Stack flight_sh
+    (requires fun h ->
+      exists from to. valid_flight_ch ch from to input h
+    )
+    (ensures fun h0 fsh h1 ->
+      B.modifies (LP.loc_slice_from_to output fsh.begin_sh fsh.end_sh) h0 h1 /\
+      LP.live_slice h1 output /\
+      valid_flight_sh fsh output h1)
+
+module LL = LowParse.Low.Base
+
+// #reset-options
+//   "--query_stats \
+//    --print_z3_statistics \
+//    --using_facts_from \
+//        '* \
+//         -TLSConstants \
+//         -Parsers \
+//         +Parsers.ClientHello \
+//         +Parsers.ServerHello \
+//         +Parsers.CipherSuite \
+//         +Parsers.Handshake' \
+//    --log_queries"
+
+assume
+val is_hrr (sh:flight_sh)
+  : Stack bool
+    (requires fun h ->
+      valid_flight_sh sh output h)
+    (ensures fun h0 b h1 ->
+      B.modifies B.loc_none h0 h1 /\
+      b == HSL.Transcript.is_hrr (Ghost.reveal sh.sh_msg))
+
+#reset-options
+  "--query_stats \
+    --print_z3_statistics \
+    --using_facts_from \
+         'Prims \
+          FStar \
+          LowStar \
+          LowParse \
+          Test.HSL.Transcript \
+          HSL \
+          CipherSuite \
+          +Hacl.Hash.Definitions
+          +Parsers.ClientHello \
+          +Parsers.ServerHello \
+          +Parsers.CipherSuite \
+          +Parsers.Handshake'"
+#set-options "--max_fuel 0"
+
+let flush (x:nat) = assert (x >= 0)
+
+module TX = HSL.Transcript
+
+assume
+val is_psk (ch:flight_ch) (from to:uint_32)
+  : Stack bool
+    (requires fun h ->
+      valid_flight_ch ch from to input h)
+    (ensures fun h0 b h1 ->
+      B.modifies B.loc_none h0 h1 /\
+      TX.client_hello_has_psk (Ghost.reveal ch.ch_msg))
+
+assume
+val truncate_at (ch:flight_ch) (from to:uint_32)
+  : Stack (uint_32 & Ghost.erased LL.bytes)
+    (requires fun h ->
+      valid_flight_ch ch from to input h /\
+      TX.client_hello_has_psk (Ghost.reveal ch.ch_msg))
+    (ensures fun h0 (i, b) h1 ->
+      B.modifies B.loc_none h0 h1 /\
+      from < i /\ i < to /\
+      Ghost.reveal b == LP.bytes_of_slice_from_to h1 input from i)
+
+#set-options "--max_ifuel 0 --z3rlimit_factor 10 --initial_ifuel 0"
+
+assume
+val check_binder
+    (#a:_)
+    (ch:flight_ch)
+    (tag:Hacl.Hash.Definitions.hash_t a)
+    (chosen_psk_identity:Parsers.PskBinderEntry.pskBinderEntry)
+ : Stack bool
+   (requires fun h0 ->
+     B.live h0 tag)
+   (ensures fun h0 _ h1 ->
+     B.modifies B.loc_none h0 h1)
+
+assume
+val select_psk_binder_entry
+      (ch:flight_ch) (from to:uint_32) (sh:flight_sh)
+   : Stack Parsers.PskBinderEntry.pskBinderEntry
+     (requires fun h0 ->
+       valid_flight_ch ch from to input h0 /\
+       valid_flight_sh sh output h0)
+     (ensures fun h0 p h1 ->
+       B.modifies B.loc_none h0 h1 /\
+       True //maybe say that p is actually in ch?
+       )
+
+assume
+val hash_len (a:_)
+  : Tot (x:uint_32{ UInt32.v x == Spec.Hash.Definitions.hash_length a })
+
+inline_for_extraction
+let new_tag (a:_) :
+  StackInline (Hacl.Hash.Definitions.hash_t a)
+    (requires fun h0 -> True)
+    (ensures fun h0 t h1 ->
+      B.modifies B.loc_none h0 h1 /\
+      B.live h1 t /\
+      B.fresh_loc (B.loc_buffer t) h0 h1)
+  = B.malloca 0uy (hash_len a)
+
+#set-options "--z3rlimit_factor 30"
+let server (from to:uint_32)
+  : ST unit
+    (requires fun h ->
+      LP.live_slice h input /\
+      LP.live_slice h output)
+    (ensures fun h0 _ h1 ->
+      B.modifies (LP.loc_slice_from output 0ul) h0 h1)
+  = push_frame();
+    let ch = receive_client_hello from to in
+    let sh = nego ch in
+    let cipherSuite_pos =
+        Parsers.ServerHello.accessor_serverHello_cipher_suite
+          output
+          sh.begin_sh
+    in
+    let cipherSuite : Parsers.CipherSuite.cipherSuite =
+      Parsers.CipherSuite.cipherSuite_reader
+        output
+        cipherSuite_pos
+    in
+    let _ =
+    match CipherSuite.cipherSuite'_of_name cipherSuite with
+    | Some (CipherSuite.CipherSuite13 _ hash_alg) ->
+      let h = get () in
+      let thash, tx_0 = TX.create Mem.tls_region hash_alg in
+      let h1 = get () in
+      if is_hrr sh
+      then begin
+        let tx_1 = HSL.Transcript.extend_hrr thash input from to output sh.begin_hsm sh.end_sh tx_0 in
+        assert (Ghost.reveal tx_1 == TX.Start (Some (Ghost.reveal ch.ch_msg, Ghost.reveal sh.sh_msg)));
+        ()
+      end
+      else begin
+        if is_psk ch from to
+        then let tch_i, tch_b = truncate_at ch from to in
+             let tx_1 = TX.extend_tch thash input from tch_i tx_0 in
+             assert (Ghost.reveal tx_1 == TX.TruncatedClientHello None (Ghost.reveal tch_b));
+             let h = get () in
+             TX.elim_invariant thash (Ghost.reveal tx_1) h;
+//             assert (TX.invariant thash (Ghost.reveal tx_1) h);
+             // assume (B.loc_not_unused_in h `B.loc_includes` TX.footprint thash);
+             let tag = new_tag hash_alg in
+             B.loc_unused_in_not_unused_in_disjoint h;
+             assert (B.loc_unused_in h `B.loc_disjoint` B.loc_not_unused_in h);
+             assert (B.loc_unused_in h `B.loc_includes` B.loc_buffer tag);
+             B.loc_disjoint_includes
+               (B.loc_unused_in h)
+               (B.loc_not_unused_in h)
+               (B.loc_buffer tag)
+               (TX.footprint thash);
+             TX.extract_hash thash tag tx_1;
+             let psk = select_psk_binder_entry ch from to sh in
+             let h2 = get () in
+             if check_binder ch tag psk
+             then ()
+             else ()
+      end
+
+    | _ -> ()
+    in
+    pop_frame ()
+
+
+    //   else begin
+    //       if is_psk ch
+    //       then let tx = TX.extend_tch thash input from (compute_tch_index input ch) in
+    //            let tch_hash = extract thash in
+    //            if not (binder.verify tch_hash (get_selected_binder ch sh.selected_binder))
+    //            then Error
+    //            else let tx = extend_tch_binders input (compute_tch_index input ch) to in
+    //               //state of thash = hash ch
+    //                 tx
+    //      else extend_hash_hsm input from to  //state of hash = hash ch
+    //     in
+
+    //   end
+    // | _ -> ()
+
+    //     let tx =
+    //       if is_psk ch sh
+    //       then let tx = extend_tch thash input from (compute_tch_index input ch) in
+    //            let tch_hash = extract thash in
+    //            if not (binder.verify tch_hash (get_selected_binder ch sh.selected_binder))
+    //            then Error
+    //            else let tx = extend_tch_binders input (compute_tch_index input ch) to in
+    //               //state of thash = hash ch
+    //                 tx
+    //      else extend_hash_hsm input from to  //state of hash = hash ch
+    //     in
+    //     let tx = extend_hash_hsm13 output sh.begin_hsm sh.end_sh in
+    //     ()
+
+
+    // | _ -> ()
+
+
+// //     | _ ->
+// //       Error
+
+//     | _ -> ()
+
+// let flush2 (x:nat) = assert (x >= 0)
+// let flush3 (x:nat) = assert (x >= 0)
+
+
+// // --------------------------------------------------------------------------------
+
+// //  ch = [ prefix ; id1..idn; b1...bn ]
+
+// //  tch = [ prefix ; id1..idn]
+
+// //  bi = HMAC(binder_key_i, tch)
+
+
+
+// // // let server2 (from to:uint_32)
+// // //   : ST unit
+// // //     (requires fun h ->
+// // //       LP.live_slice h input /\
+// // //       LP.live_slice h output)
+// // //     (ensures fun h0 _ h1 ->
+// // //       B.modifies (LP.loc_slice_from output 0ul) h0 h1)
+// // //   = let ch = receive_client_hello from to in
+// // //     let sh = nego ch in
+// // //     let h0 = get () in
+// // //     // assert (LP.valid_pos HSM.handshake_parser h0 output sh.begin_hsm sh.end_sh);
+// // // //    assert (trigger (LP.get_valid_pos HSM.handshake_parser h0 output sh.begin_hsm));
+// // //       let cipherSuite_pos =
+// // //         Parsers.ServerHello.accessor_serverHello_cipher_suite
+// // //           output
+// // //           sh.begin_sh
+// // //       in
+// // //       let h1 = get () in
+// // //       //LL.valid_frame HSM.handshake_parser h0 output sh.begin_hsm B.loc_none h1;
+// // //       // assume (LP.valid_content_pos HSM.handshake_parser h1 output sh.begin_hsm
+// // //       //                              (LP.contents HSM.handshake_parser h0 output sh.begin_hsm)
+// // //       //                              sh.end_sh);
+// // //       // assert (sh.end_sh == LP.get_valid_pos HSM.handshake_parser h1 output sh.begin_hsm);
+// // //       // assert (LP.valid_pos HSM.handshake_parser h1 output sh.begin_hsm sh.end_sh);
+// // //       // admit()
+// // //       // test_frame HSM.handshake_parser h0 sh.begin_hsm B.loc_none h1;
+// // //       // assert (LP.valid HSM.handshake_parser h0 output sh.begin_hsm);
+// // //       // assert (B.modifies B.loc_none h0 h1);
+// // //       assert (LP.valid_pos HSM.handshake_parser h1 output sh.begin_hsm sh.end_sh)
+
+
+// // let server3 (from to:uint_32)
+// //   : ST unit
+// //     (requires fun h ->
+// //       LP.live_slice h input /\
+// //       LP.live_slice h output)
+// //     (ensures fun h0 _ h1 ->
+// //       B.modifies (LP.loc_slice_from output 0ul) h0 h1)
+// //   = let ch = receive_client_hello from to in
+// //     let sh = nego ch in
+// //     let h0 = get () in
+// //     // assert (LP.valid_pos HSM.handshake_parser h0 output sh.begin_hsm sh.end_sh);
+// // //    assert (trigger (LP.get_valid_pos HSM.handshake_parser h0 output sh.begin_hsm));
+// //       let cipherSuite_pos =
+// //         Parsers.ServerHello.accessor_serverHello_cipher_suite
+// //           output
+// //           sh.begin_sh
+// //       in
+// //       let h1 = get () in
+// //       //LL.valid_frame HSM.handshake_parser h0 output sh.begin_hsm B.loc_none h1;
+// //       // assume (LP.valid_content_pos HSM.handshake_parser h1 output sh.begin_hsm
+// //       //                              (LP.contents HSM.handshake_parser h0 output sh.begin_hsm)
+// //       //                              sh.end_sh);
+// //       // assert (sh.end_sh == LP.get_valid_pos HSM.handshake_parser h1 output sh.begin_hsm);
+// //       // assert (LP.valid_pos HSM.handshake_parser h1 output sh.begin_hsm sh.end_sh);
+// //       // admit()
+// //       // test_frame HSM.handshake_parser h0 sh.begin_hsm B.loc_none h1;
+// //       // assert (LP.valid HSM.handshake_parser h0 output sh.begin_hsm);
+// //       // assert (B.modifies B.loc_none h0 h1);
+// //       assert (LP.valid_pos HSM.handshake_parser h1 output sh.begin_hsm sh.end_sh)
+
+
+// // let server4 (from to:uint_32)
+// //   : ST unit
+// //     (requires fun h ->
+// //       LP.live_slice h input /\
+// //       LP.live_slice h output)
+// //     (ensures fun h0 _ h1 ->
+// //       B.modifies (LP.loc_slice_from output 0ul) h0 h1)
+// //   = let ch = receive_client_hello from to in
+// //     let sh = nego ch in
+// //     let h0 = get () in
+// //     // assert (LP.valid_pos HSM.handshake_parser h0 output sh.begin_hsm sh.end_sh);
+// // //    assert (trigger (LP.get_valid_pos HSM.handshake_parser h0 output sh.begin_hsm));
+// //       let cipherSuite_pos =
+// //         Parsers.ServerHello.accessor_serverHello_cipher_suite
+// //           output
+// //           sh.begin_sh
+// //       in
+// //       let h1 = get () in
+// //       //LL.valid_frame HSM.handshake_parser h0 output sh.begin_hsm B.loc_none h1;
+// //       // assume (LP.valid_content_pos HSM.handshake_parser h1 output sh.begin_hsm
+// //       //                              (LP.contents HSM.handshake_parser h0 output sh.begin_hsm)
+// //       //                              sh.end_sh);
+// //       // assert (sh.end_sh == LP.get_valid_pos HSM.handshake_parser h1 output sh.begin_hsm);
+// //       // assert (LP.valid_pos HSM.handshake_parser h1 output sh.begin_hsm sh.end_sh);
+// //       // admit()
+// //       // test_frame HSM.handshake_parser h0 sh.begin_hsm B.loc_none h1;
+// //       // assert (LP.valid HSM.handshake_parser h0 output sh.begin_hsm);
+// //       // assert (B.modifies B.loc_none h0 h1);
+// //       assert (LP.valid_pos HSM.handshake_parser h1 output sh.begin_hsm sh.end_sh)
+
+// // #reset-options
+// //   "--query_stats \
+// //     --print_z3_statistics \
+// //     --log_queries \
+// //     --using_facts_from \
+// //          '* \
+// //           -TLSConstants \
+// //           -Parsers \
+// //           +Parsers.ClientHello \
+// //           +Parsers.ServerHello \
+// //           +Parsers.CipherSuite \
+// //           +Parsers.Handshake'"
+
+// // let server5 (from to:uint_32)
+// //   : ST unit
+// //     (requires fun h ->
+// //       LP.live_slice h input /\
+// //       LP.live_slice h output)
+// //     (ensures fun h0 _ h1 ->
+// //       B.modifies (LP.loc_slice_from output 0ul) h0 h1)
+// //   = let ch = receive_client_hello from to in
+// //     let sh = nego ch in
+// //     let h0 = get () in
+// //     // assert (LP.valid_pos HSM.handshake_parser h0 output sh.begin_hsm sh.end_sh);
+// // //    assert (trigger (LP.get_valid_pos HSM.handshake_parser h0 output sh.begin_hsm));
+// //       let cipherSuite_pos =
+// //         Parsers.ServerHello.accessor_serverHello_cipher_suite
+// //           output
+// //           sh.begin_sh
+// //       in
+// //       let h1 = get () in
+// //       //LL.valid_frame HSM.handshake_parser h0 output sh.begin_hsm B.loc_none h1;
+// //       // assume (LP.valid_content_pos HSM.handshake_parser h1 output sh.begin_hsm
+// //       //                              (LP.contents HSM.handshake_parser h0 output sh.begin_hsm)
+// //       //                              sh.end_sh);
+// //       // assert (sh.end_sh == LP.get_valid_pos HSM.handshake_parser h1 output sh.begin_hsm);
+// //       // assert (LP.valid_pos HSM.handshake_parser h1 output sh.begin_hsm sh.end_sh);
+// //       // admit()
+// //       // test_frame HSM.handshake_parser h0 sh.begin_hsm B.loc_none h1;
+// //       // assert (LP.valid HSM.handshake_parser h0 output sh.begin_hsm);
+// //       // assert (B.modifies B.loc_none h0 h1);
+// //       assert (LP.valid_pos HSM.handshake_parser h1 output sh.begin_hsm sh.end_sh)
+
+
+
+// // let test4 (x:nat) = assert (x >= 0)
+// //     //   ;
+// //     //   admit()
+// //     // let cipherSuite : Parsers.CipherSuite.cipherSuite =
+// //     //   Parsers.CipherSuite.cipherSuite_reader
+// //     //     output
+// //     //     cipherSuite_pos
+// //     // in
+// //     // match CipherSuite.cipherSuite'_of_name cipherSuite with
+// //     // | Some (CipherSuite.CipherSuite13 _ hash_alg) ->
+// //     //   let h = get () in
+// //     //   assert (valid_flight_sh sh output h);
+// //     //   admit();
+// //     //   let tx = HSL.Transcript.create Mem.tls_region hash_alg in
+// //     //   if is_hrr sh
+// //     //   then ()
+// //     //   else ()
+// //     // | _ ->
+// //     //   ()
